NS/TypesSubtype.v
@@ -10,7 +10,9 @@ Require Import Coq.Logic.Eqdep.
 Require Import Coq.Program.Equality.
 Require Import Coq.Relations.Relation_Definitions.
 Require Import Lia.
+Require Import LibHyps.LibHyps.
 From NS Require Import Misc.
+From NS Require Import HigherOrder.
 From NS Require Import JsRecord.
 From NS Require Import TypesBase.
 From NS Require Import TypesNotation.
@@ -24,6 +26,8 @@ Local Notation "a >= b" := (Bool.le b a) : bool_scope.
 
 (* Subtype relation *)
 Class Subtype (A: Set) := subtype: relation A.
+Class Subtype1 (F: Set -> Set) := subtype1: forall {A: Set}, relation A -> relation (F A).
+Global Instance unSubtype1 {F: Set -> Set} {C1: Subtype1 F} {A: Set} {C: Subtype A}: Subtype (F A) := subtype1 C.
 (* Definition wrapper prevents Coq from printing everything as a subtype relation
    while still printing explicitly defined subtype relations *)
 Definition ap_Subtype {A: Set} (S: Subtype A) (lhs rhs: A) := S lhs rhs.
@@ -52,22 +56,42 @@ Notation "'(I)'" := Intersection.
 Notation "lhs 'I' rhs '=' a" := (Intersection lhs rhs a) (at level 60, rhs at next level, no associativity).
 
 Class EqvType (A: Set) := eqv_type: relation A.
+Class EqvType1 (F: Set -> Set) := eqv_type1: forall {A: Set}, relation A -> relation (F A).
+Global Instance unEqvType1 {F: Set -> Set} {C1: EqvType1 F} {A: Set} {C: EqvType A}: EqvType (F A) := eqv_type1 C.
 Definition ap_EqvType {A: Set} (S: EqvType A) (lhs rhs: A) := S lhs rhs.
 Notation "'[' eqv_type ']' lhs '==' rhs" := (ap_EqvType eqv_type lhs rhs) (at level 60, lhs at next level, rhs at next level, no associativity).
 Notation "lhs '==' rhs" := (eqv_type lhs rhs) (at level 60, rhs at next level, no associativity).
 
 Class IsValidType (A: Set) := is_valid_type: A -> Prop.
+Class IsValidType1 (F: Set -> Set) := is_valid_type1: forall {A: Set}, (A -> Prop) -> (F A -> Prop).
+Global Instance unIsValidType1 {F: Set -> Set} {C1: IsValidType1 F} {A: Set} {C: IsValidType A}: IsValidType (F A) := is_valid_type1 C.
+Definition unIsValidType1' {F: Set -> Set} {A: Set} `{C1: IsValidType1 F} `{C: IsValidType A}: forall a, is_valid_type1 C a -> is_valid_type a.
+  intros; unfold is_valid_type, unIsValidType1; exact H. Defined.
 Definition IsValidType_always {A: Set}: IsValidType A := fun _ => True.
 
 (* Subtype properties *)
 Unset Implicit Arguments.
 Class Top (A: Set): Set := top: A.
+Class Top1 (F: Set -> Set) := top1: forall {A: Set}, Top A -> F A.
+Global Instance unTop1 {F: Set -> Set} {C1: Top1 F} {A: Set} {C: Top A}: Top (F A) := top1 C.
 Class Bottom (A: Set): Set := bottom: A.
+Class Bottom1 (F: Set -> Set) := bottom1: forall {A: Set}, Bottom A -> F A.
+Global Instance unBottom1 {F: Set -> Set} {C1: Bottom1 F} {A: Set} {C: Bottom A}: Bottom (F A) := bottom1 C.
 Class SubtypeTop (A: Set) `{_Subtype: Subtype A} `{_Top: Top A}: Prop := subtype_top: forall (a: A), a <: top.
+Class SubtypeTop1 (F: Set -> Set) `{_Subtype1: Subtype1 F} `{_Top1: Top1 F}: Prop := subtype_top1: forall {A: Set} `{_Subtype: Subtype A} `{_Top: Top A}, SubtypeTop A -> SubtypeTop (F A).
+Global Instance unSubtypeTop1 {F: Set -> Set} `{C1: SubtypeTop1 F} {A: Set} `{C: SubtypeTop A}: SubtypeTop (F A) := subtype_top1 C.
 Class SubtypeBottom (A: Set) `{_Subtype: Subtype A} `{_Bottom: Bottom A}: Prop := subtype_bottom: forall (a: A), bottom <: a.
+Class SubtypeBottom1 (F: Set -> Set) `{_Subtype1: Subtype1 F} `{_Bottom1: Bottom1 F}: Prop := subtype_bottom1: forall {A: Set} {_Subtype: Subtype A} {_Bottom: Bottom A}, SubtypeBottom A -> SubtypeBottom (F A).
+Global Instance unSubtypeBottom1 {F: Set -> Set} `{C1: SubtypeBottom1 F} {A: Set} `{C: SubtypeBottom A}: SubtypeBottom (F A) := subtype_bottom1 C.
 Class SubtypeRefl (A: Set) `{_Subtype: Subtype A} `{_IsValidType: IsValidType A}: Prop := subtype_refl: forall (a: A), is_valid_type a -> a <: a.
+Class SubtypeRefl1 (F: Set -> Set) `{_Subtype1: Subtype1 F} `{_IsValidType1: IsValidType1 F}: Prop := subtype_refl1: forall {A: Set} `{_Subtype: Subtype A} `{_IsValidType: IsValidType A}, SubtypeRefl A -> SubtypeRefl (F A).
+Global Instance unSubtypeRefl1 {F: Set -> Set} `{C1: SubtypeRefl1 F} {A: Set} `{C: SubtypeRefl A}: SubtypeRefl (F A) := subtype_refl1 C.
 Class SubtypeAntisym (A: Set) `{_Subtype: Subtype A} `{_EqvType: EqvType A}: Prop := subtype_antisym: forall (a b: A), a <: b -> b <: a -> a == b.
+Class SubtypeAntisym1 (F: Set -> Set) `{_Subtype1: Subtype1 F} `{_EqvType1: EqvType1 F}: Prop := subtype_antisym1: forall {A: Set} `{_Subtype: Subtype A} `{_EqvType: EqvType A}, SubtypeAntisym A -> SubtypeAntisym (F A).
+Global Instance unSubtypeAntisym1 {F: Set -> Set} `{C1: SubtypeAntisym1 F} {A: Set} `{C: SubtypeAntisym A}: SubtypeAntisym (F A) := subtype_antisym1 C.
 Class SubtypeTrans (A: Set) `{_Subtype: Subtype A}: Prop := subtype_trans: forall (a b c: A), a <: b -> b <: c -> a <: c.
+Class SubtypeTrans1 (F: Set -> Set) `{_Subtype1: Subtype1 F}: Prop := subtype_trans1: forall {A: Set} `{_Subtype: Subtype A}, SubtypeTrans A -> SubtypeTrans (F A).
+Global Instance unSubtypeTrans1 {F: Set -> Set} `{C1: SubtypeTrans1 F} {A: Set} `{C: SubtypeTrans A}: SubtypeTrans (F A) := subtype_trans1 C.
 Class SubtypeValid (A: Set) `{_Subtype: Subtype A} `{_IsValidType: IsValidType A} `{_EqvType: EqvType A}: Prop := subtype_valid: SubtypeRefl A /\ SubtypeAntisym A /\ SubtypeTrans A.
 Class SubtypeValid0 (A: Set) `{_Subtype: Subtype A} `{_IsValidType: IsValidType A} `{_EqvType: EqvType A} `{_Top: Top A} `{_Bottom: Bottom A}: Prop := subtype_valid0: SubtypeTop A /\ SubtypeBottom A /\ SubtypeValid A.
 (* TODO: Some of these = may need to be == *)
@@ -100,25 +124,31 @@ Inductive S_option {A: Set} (S: Subtype A): Subtype (option A) :=
 | S_None            : forall (lhs: option A), [S_option S] lhs <: None
 | S_Some            : forall (lhs rhs: A), [S] lhs <: rhs -> [S_option S] Some lhs <: Some rhs
 . Global Instance SOf_option {A: Set} {S: Subtype A}: Subtype (option A) := S_option S.
+Global Instance S1Of_option: Subtype1 option := @S_option.
 Inductive E_option {A: Set} (E: EqvType A) : EqvType (option A) :=
 | E_None            : forall (lhs: option A), [E_option E] lhs == None
 | E_Some            : forall (lhs rhs: A), [E] lhs == rhs -> [E_option E] (Some lhs) == (Some rhs)
 . Global Instance EOf_option {A: Set} {E: EqvType A}: EqvType (option A) := E_option E.
+Global Instance E1Of_option: EqvType1 option := @E_option.
 Inductive S_Zip {A: Set} (S: Subtype A): Subtype (list A) :=
 | S_Zip_nil          : forall (lhs: list A), [S_Zip S] lhs <: nil
 | S_Zip_cons         : forall (l r: A) (ls rs: list A),
     [S] l <: r -> [S_Zip S] ls <: rs -> [S_Zip S] (l :: ls) <: (r :: rs)
 (* no global instance because there is S_Intersect *)
 . Definition SOf_Zip {A: Set} {S: Subtype A}: Subtype (list A) := S_Zip S.
+Definition S1Of_Zip: Subtype1 list := @S_Zip.
 Inductive E_Zip {A: Set} (E: EqvType A) : EqvType (list A) :=
 | E_Zip_nil          : [E_Zip E] nil == nil
 | E_Zip_cons         : forall (l r: A) (ls rs: list A),
     [E] l == r -> [E_Zip E] ls == rs -> [E_Zip E] (l :: ls) == (r :: rs)
 . Global Instance EOf_Zip {A: Set} {E: EqvType A}: EqvType (list A) := E_Zip E.
+Global Instance E1Of_Zip: EqvType1 list := @E_Zip.
 (* no global instance because there is S_Zip and S_Intersect *)
 Definition S_JsrZip {A: Set} (S: Subtype A): Subtype (js_record A) := JsRecord1Rel S.
 Definition SOf_JsrZip {A: Set} {S: Subtype A}: Subtype (js_record A) := JsRecord1Rel S.
+Definition S1Of_JsrZip: Subtype1 js_record := @S_JsrZip.
 Global Instance EOf_JsrZip {A: Set} {E: EqvType A}: EqvType (js_record A) := JsRecordRel E.
+Global Instance E1Of_JsrZip: EqvType1 js_record := @EOf_JsrZip.
 Inductive S_Intersect {A: Set} (S: Subtype A): Subtype (list A) :=
 | S_Intersect_nil    : forall (lhs: list A), [S_Intersect S] lhs <: nil
 | S_Intersect_cons   : forall (l r: A) (ls rs: list A),
@@ -127,6 +157,7 @@ Inductive S_Intersect {A: Set} (S: Subtype A): Subtype (list A) :=
                  [S_Intersect S] ls <: rs -> [S_Intersect S] (l :: ls) <: rs
 (* no global instance because there is S_Zip *)
 . Definition SOf_Intersect {A: Set} {S: Subtype A}: Subtype (list A) := S_Intersect S.
+Definition S1Of_Intersect: Subtype1 list := @S_Intersect.
 Inductive S_variance: Subtype variance :=
 | S_Bivariant        : forall (lhs: variance), [S_variance] lhs <: Bivariant
 | S_Covariant        : [S_variance] Covariant <: Covariant
@@ -137,32 +168,40 @@ Global Instance EOf_variance: EqvType variance := eq.
 Inductive S_otype {A: Set} (S: Subtype A): Subtype (otype A) :=
 | S_OType            : forall (ol or: bool) (lhs rhs: A), ol <= or -> [S] lhs <: rhs -> [S_otype S] Ot ol lhs <: Ot or rhs
 . Global Instance SOf_otype {A: Set} {S: Subtype A}: Subtype (otype A) := S_otype S.
+Global Instance S1Of_otype: Subtype1 otype := @S_otype.
 Inductive E_otype {A: Set} (E: EqvType A): EqvType (otype A) :=
 | E_OType            : forall (o: bool) (lhs rhs: A), [E] lhs == rhs -> [E_otype E] Ot o lhs == Ot o rhs
 . Global Instance EOf_otype {A: Set} {E: EqvType A}: EqvType (otype A) := E_otype E.
+Global Instance E1Of_otype: EqvType1 otype := @E_otype.
 Inductive S_vtype {A: Set} (S: Subtype A): Subtype (vtype A) :=
 | S_Void             : [S_vtype S] @VVoid A <: VVoid
 | S_NotVoid          : forall (lhs rhs: A), [S] lhs <: rhs -> [S_vtype S] Vt lhs <: Vt rhs
 . Global Instance SOf_vtype {A: Set} {S: Subtype A}: Subtype (vtype A) := S_vtype S.
+Global Instance S1Of_vtype: Subtype1 vtype := @S_vtype.
 Inductive E_vtype {A: Set} (E: EqvType A): EqvType (vtype A) :=
 | E_Void             : [E_vtype E] @VVoid A == VVoid
 | E_NotVoid          : forall (lhs rhs: A), [E] lhs == rhs -> [E_vtype E] Vt lhs == Vt rhs
 . Global Instance EOf_vtype {A: Set} {E: EqvType A}: EqvType (vtype A) := E_vtype E.
+Global Instance E1Of_vtype: EqvType1 vtype := @E_vtype.
 Inductive S_tparam {A: Set} (S: Subtype A): Subtype (tparam A) :=
 | S_TParam           : forall (vl vr: variance) (name: string) (supl supr: list A),
     [S_variance] vl <: vr -> [S_Intersect S] supl <: supr ->
     [S_tparam S] TParam vl name supl <: TParam vr name supr
 . Global Instance SOf_tparam {A: Set} {S: Subtype A}: Subtype (tparam A) := S_tparam S.
+Global Instance S1Of_tparam: Subtype1 tparam := @S_tparam.
 Inductive E_tparam {A: Set} (E: EqvType A): EqvType (tparam A) :=
 | E_TParam           : forall (v: variance) (name: string) (supl supr: list A),
     [E_Zip E] supl == supr -> [E_tparam E] TParam v name supl == TParam v name supr
 . Global Instance EOf_tparam {A: Set} {E: EqvType A}: EqvType (tparam A) := E_tparam E.
+Global Instance E1Of_tparam: EqvType1 tparam := @E_tparam.
 Inductive S_itype {A: Set} (S: Subtype A): Subtype (itype A) :=
 | S_Ident            : forall (name: string) (tal tar: list A), [S_Zip S] tal <: tar -> [S_itype S] It name tal <: It name tar
 . Global Instance SOf_itype {A: Set} {S: Subtype A}: Subtype (itype A) := S_itype S.
+Global Instance S1Of_itype: Subtype1 itype := @S_itype.
 Inductive E_itype {A: Set} (E: EqvType A): EqvType (itype A) :=
 | E_Ident            : forall (name: string) (tal tar: list A), [E_Zip E] tal == tar -> [E_itype E] It name tal == It name tar
 . Global Instance EOf_itype {A: Set} {E: EqvType A}: EqvType (itype A) := E_itype E.
+Global Instance E1Of_itype: EqvType1 itype := @E_itype.
 Inductive S_stype {A: Set} (S: Subtype A): Subtype (stype A) :=
 | S_Fn               : forall (tpl tpr: list (tparam A)) (thispl thispr: A)
                          (pl pr: list (otype A)) (rl rr: A) (retl retr: (vtype A)),
@@ -172,6 +211,7 @@ Inductive S_stype {A: Set} (S: Subtype A): Subtype (stype A) :=
 | S_Tuple            : forall (esl esr: list (otype A)),      [S_Zip (S_otype S)]    esl <: esr -> [S_stype S] STuple esl  <: STuple esr
 | S_Object           : forall (fsl fsr: js_record (otype A)), [S_JsrZip (S_otype S)] fsl <: fsr -> [S_stype S] SObject fsl <: SObject fsr
 . Global Instance SOf_stype {A: Set} {S: Subtype A}: Subtype (stype A) := S_stype S.
+Global Instance S1Of_stype: Subtype1 stype := @S_stype.
 Inductive E_stype {A: Set} (E: EqvType A): EqvType (stype A) :=
 | E_Fn               : forall (tpl tpr: list (tparam A)) (thispl thispr: A)
                          (pl pr: list (otype A)) (rl rr: A) (retl retr: (vtype A)),
@@ -181,6 +221,7 @@ Inductive E_stype {A: Set} (E: EqvType A): EqvType (stype A) :=
 | E_Tuple            : forall (esl esr: list (otype A)),      [E_Zip (E_otype E)]    esl == esr -> [E_stype E] STuple esl  == STuple esr
 | E_Object           : forall (fsl fsr: js_record (otype A)), [JsRecordRel (E_otype E)] fsl == fsr -> [E_stype E] SObject fsl == SObject fsr
 . Global Instance EOf_stype {A: Set} {E: EqvType A}: EqvType (stype A) := E_stype E.
+Global Instance E1Of_stype: EqvType1 stype := @E_stype.
 Inductive S_ftype: Subtype ftype :=
 | S_Any              : forall (lhs: ftype), [S_ftype] lhs <: FAny
 | S_Never            : forall (rhs: ftype), [S_ftype] FNEVER <: rhs
@@ -237,43 +278,43 @@ Axiom E_ftype_ind':
     (lhs rhs: ftype), E_ftype lhs rhs -> P lhs rhs.
 
 (* Now we prove that these relations are valid *)
-Global Instance Top_option {A: Set} `{_Top: Top A}: Top (option A) := None.
-Global Instance Bottom_option {A: Set} `{_Bottom: Bottom A}: Bottom (option A) := Some bottom.
-Global Instance IsValidType_option {A: Set} `{V: IsValidType A}: IsValidType (option A) := Option_Forall V.
-Global Instance SubtypeRefl_option {A: Set} `(_SubtypeRefl: SubtypeRefl A): SubtypeRefl (option A).
-Proof. intros a; destruct a; constructor; apply subtype_refl; inv H; assumption. Qed.
-Global Instance SubtypeAntisym_option {A: Set} `(_SubtypeAntisym: SubtypeAntisym A): SubtypeAntisym (option A).
-Proof. intros a b H H0; destruct a, b; inv H H0; constructor; apply subtype_antisym; assumption. Qed.
-Global Instance SubtypeTrans_option {A: Set} `{_SubtypeTrans: SubtypeTrans A}: SubtypeTrans (option A).
-Proof. intros a b c H H0; destruct a, b, c; inv H H0; constructor; apply subtype_trans with a0; assumption. Qed.
+Global Instance Top_option: Top1 option := fun _ _ => None.
+Global Instance Bottom_option: Bottom1 option := @Some.
+Global Instance IsValidType_option: IsValidType1 option := @Option_Forall.
+Global Instance SubtypeRefl_option: SubtypeRefl1 option.
+Proof. intros A S V C a; destruct a; constructor; apply subtype_refl; inv H; assumption. Qed.
+Global Instance SubtypeAntisym_option: SubtypeAntisym1 option.
+Proof. intros A S E C a b H H0; destruct a, b; inv H H0; constructor; apply subtype_antisym; assumption. Qed.
+Global Instance SubtypeTrans_option: SubtypeTrans1 option.
+Proof. intros A S C a b c H H0; destruct a, b, c; inv H H0; constructor; apply subtype_trans with a0; assumption. Qed.
 
-Global Instance IsValidType_list {A: Set} `{V: IsValidType A}: IsValidType (list A) := List.Forall V.
-Global Instance SubtypeRefl_Zip {A: Set} `{_SubtypeRefl: SubtypeRefl A}: @SubtypeRefl (list A) SOf_Zip IsValidType_list.
-Proof. intros a; induction a; constructor; [apply subtype_refl | apply IHa]; inv H; assumption. Qed.
-Global Instance SubtypeAntisym_Zip {A: Set} `{_SubtypeAntisym: SubtypeAntisym A}: @SubtypeAntisym (list A) SOf_Zip EOf_Zip.
-Proof. intros a b H H0; (induction2 a b using ind_list2); [inv H H0 | inv H0 H1 .. ]; constructor; [apply subtype_antisym | apply H]; assumption. Qed.
-Global Instance SubtypeTrans_Zip {A: Set} `{_SubtypeTrans: SubtypeTrans A}: @SubtypeTrans (list A) SOf_Zip.
-Proof. intros a b c H H0; (induction3 a b c using ind_list3); [inv H H0 | inv H0 H1 ..]; constructor; [apply subtype_trans with y | apply H]; assumption. Qed.
+Global Instance IsValidType_list: IsValidType1 list := @List.Forall.
+Global Instance SubtypeRefl_Zip: @SubtypeRefl1 list S1Of_Zip IsValidType_list.
+Proof. intros A S V C a; induction a; constructor; [apply subtype_refl | apply IHa]; inv H; assumption. Qed.
+Global Instance SubtypeAntisym_Zip: @SubtypeAntisym1 list S1Of_Zip E1Of_Zip.
+Proof. intros A S E C a b H H0; (induction2 a b using ind_list2); [inv H H0 | inv H0 H1 .. ]; constructor; [apply subtype_antisym | apply H]; assumption. Qed.
+Global Instance SubtypeTrans_Zip: @SubtypeTrans1 list S1Of_Zip.
+Proof. intros A S C a b c H H0; (induction3 a b c using ind_list3); [inv H H0 | inv H0 H1 ..]; constructor; [apply subtype_trans with y | apply H]; assumption. Qed.
 
-Global Instance IsValidType_js_record {A: Set} `{V: IsValidType A}: IsValidType (js_record A) := JsRecordNoDupForall V.
-Global Instance SubtypeRefl_JsrZip {A: Set} `{_SubtypeRefl: SubtypeRefl A}: @SubtypeRefl (js_record A) SOf_JsrZip IsValidType_js_record.
-Proof. intros a; induction a; [constructor; constructor |]; destruct a as [ka va]; intros; apply JsRecord1Rel_cons with va a0; [apply subtype_refl | apply IHa | apply JsRecordAdd_head |]; inv H; assumption. Qed.
-Global Instance SubtypeAntisym_JsrZip {A: Set} `{_SubtypeAntisym: SubtypeAntisym A}: @SubtypeAntisym (js_record A) SOf_JsrZip EOf_JsrZip.
+Global Instance IsValidType_js_record: IsValidType1 js_record := @JsRecordNoDupForall.
+Global Instance SubtypeRefl_JsrZip: @SubtypeRefl1 js_record S1Of_JsrZip IsValidType_js_record.
+Proof. intros A S V C a; induction a; [constructor; constructor |]; destruct a as [ka va]; intros; apply JsRecord1Rel_cons with va a0; [apply subtype_refl | apply IHa | apply JsRecordAdd_head |]; inv H; assumption. Qed.
+Global Instance SubtypeAntisym_JsrZip: @SubtypeAntisym1 js_record S1Of_JsrZip E1Of_JsrZip.
 Proof.
-  intros a b H H0; pose (JsRecord1Rel_In H); pose (JsRecord1Rel_In H0); apply JsRecordRel_In0; try assumption.
+  intros A S E C a b H H0; pose (JsRecord1Rel_In H); pose (JsRecord1Rel_In H0); apply JsRecordRel_In0; try assumption.
   - eapply proj1, JsRecord1Rel_NoDup; exact H.
   - eapply proj1, JsRecord1Rel_NoDup; exact H0.
-  - split; intros; [apply (@JsRecord1Rel_HasKey A _Subtype) with a | apply (@JsRecord1Rel_HasKey A _Subtype) with b]; assumption.
-  - intros; apply subtype_antisym; [apply _s with k | apply _s0 with k]; assumption.
+  - split; intros; [apply (@JsRecord1Rel_HasKey A S) with a | apply (@JsRecord1Rel_HasKey A S) with b]; assumption.
+  - intros; apply subtype_antisym; [apply s with k | apply s0 with k]; assumption.
 Qed.
-Global Instance SubtypeTrans_JsrZip {A: Set} `{_SubtypeTrans: SubtypeTrans A}: @SubtypeTrans (js_record A) SOf_JsrZip.
+Global Instance SubtypeTrans_JsrZip: @SubtypeTrans1 js_record S1Of_JsrZip.
 Proof.
-  intros a b c H H0; pose (JsRecord1Rel_In H); pose (JsRecord1Rel_In H0); apply JsRecord1Rel_In0; try assumption.
+  intros A S C a b c H H0; pose (JsRecord1Rel_In H); pose (JsRecord1Rel_In H0); apply JsRecord1Rel_In0; try assumption.
   - eapply proj1, JsRecord1Rel_NoDup; exact H.
   - eapply proj2, JsRecord1Rel_NoDup; exact H0.
-  - intros; apply (@JsRecord1Rel_HasKey A _Subtype) with b, (@JsRecord1Rel_HasKey A _Subtype) with c; assumption.
-  - intros; destruct (JsRecordHasKey_dec k b); [| contradict H3; apply (@JsRecord1Rel_HasKey A _Subtype) with c; [| apply JsRecordHasKey_In0 with vy]; assumption]; rewrite JsRecordHasKey_In in H3; destruct H3 as [vb H3].
-    apply subtype_trans with vb; [apply _s with k | apply _s0 with k]; assumption.
+  - intros; apply (@JsRecord1Rel_HasKey A S) with b, (@JsRecord1Rel_HasKey A S) with c; assumption.
+  - intros; destruct (JsRecordHasKey_dec k b); [| contradict H3; apply (@JsRecord1Rel_HasKey A S) with c; [| apply JsRecordHasKey_In0 with vy]; assumption]; rewrite JsRecordHasKey_In in H3; destruct H3 as [vb H3].
+    apply subtype_trans with vb; [apply s with k | apply s0 with k]; assumption.
 Qed.
 
 Lemma S_Intersect_length {A: Set} {S: Subtype A}: forall (xs ys: list A), [S_Intersect S] xs <: ys -> (List.length ys <= List.length xs)%nat.
@@ -282,17 +323,17 @@ Lemma S_Intersect_length_antisym {A: Set} {S: Subtype A}: forall (xs ys: list A)
 Proof. intros; apply Nat.le_antisymm; apply S_Intersect_length; assumption. Qed.
 Local Ltac discr_on_intersect_length := lazymatch goal with | H: [S_Intersect _] _ <: _, H0: [S_Intersect _] _ <: _ |- _ => let e := fresh "e" in let e0 := fresh "e0" in pose' (S_Intersect_length H) as e; pose' (S_Intersect_length H0) as e0; simpl in e, e0 end; lia.
 
-Global Instance SubtypeRefl_Intersect {A: Set} `{_SubtypeRefl: SubtypeRefl A}: @SubtypeRefl (list A) SOf_Intersect IsValidType_list.
-Proof. intros a; induction a; constructor; [apply subtype_refl | apply IHa]; inv H; assumption. Qed.
-Global Instance SubtypeAntisym_Intersect {A: Set} `{_SubtypeAntisym: SubtypeAntisym A}: @SubtypeAntisym (list A) SOf_Intersect EOf_Zip.
+Global Instance SubtypeRefl_Intersect: @SubtypeRefl1 list S1Of_Intersect IsValidType_list.
+Proof. intros A S V C a; induction a; constructor; [apply subtype_refl | apply IHa]; inv H; assumption. Qed.
+Global Instance SubtypeAntisym_Intersect: @SubtypeAntisym1 list S1Of_Intersect E1Of_Zip.
 Proof.
-  intros a b H H0; pose' (S_Intersect_length_antisym H H0); (induction2 a b using ind_list2); simpl in e;
+  intros A S E C a b H H0; pose' (S_Intersect_length_antisym H H0); (induction2 a b using ind_list2); simpl in e;
     [constructor | discriminate e | discriminate e |]; inv e H0 H1; try discr_on_intersect_length;
     constructor; [apply subtype_antisym | apply H]; assumption.
 Qed.
-Global Instance SubtypeTrans_Intersect {A: Set} `{_SubtypeTrans: SubtypeTrans A}: @SubtypeTrans (list A) SOf_Intersect.
+Global Instance SubtypeTrans_Intersect: @SubtypeTrans1 list S1Of_Intersect.
 Proof.
-  intros a; induction a; try rename a into a0, a0 into a; induction b; try rename a1 into b0; induction c; try rename a1 into c0; intros;
+  intros A S C a; induction a; try rename a into a0, a0 into a; induction b; try rename a1 into b0; induction c; try rename a1 into c0; intros;
     try (inv H H0; fail); [constructor .. |]; inv H H0;
     [constructor; [apply subtype_trans with b0 | apply IHa with b] | apply IHb; [constructor |] | constructor; apply IHa with (b0 :: b); [| constructor] ..]; assumption.
 Qed.
@@ -307,80 +348,73 @@ Proof. intros a b H H0; destruct a, b; inv H H0; constructor. Qed.
 Global Instance SubtypeTrans_variance: SubtypeTrans variance.
 Proof. intros a b c H H0; destruct a, b, c; inv H H0; constructor. Qed.
 
-(* TODO rest of the relations *)
-Global Instance Top_otype {A: Set} `{_Top: Top A}: Top (otype A) := Ot true _Top.
-Global Instance Bottom_otype {A: Set} `{_Bottom: Bottom A}: Bottom (otype A) := Ot false _Bottom.
-Global Instance IsValidType_otype {A: Set} `{V: IsValidType A}: IsValidType (otype A) := fun '(Ot _ a) => V a.
-Global Instance SubtypeRefl_otype {A: Set} `{_SubtypeRefl: SubtypeRefl A}: SubtypeRefl (otype A).
-Proof. intros a; destruct a; constructor; [destruct optional; simpl; reflexivity | apply subtype_refl]; assumption. Qed.
-Global Instance SubtypeAntisym_otype {A: Set} `{_SubtypeAntisym: SubtypeAntisym A}: SubtypeAntisym (otype A).
-Proof. intros a b H H0; destruct a, b; inv H H0; destruct optional, optional0; try discriminate; constructor; apply subtype_antisym; assumption. Qed.
-Global Instance SubtypeTrans_otype {A: Set} `{_SubtypeTrans: SubtypeTrans A}: SubtypeTrans (otype A).
-Proof. intros a b c H H0; destruct a, b, c; inv H H0; destruct optional, optional0, optional1; try discriminate; constructor; (simpl; reflexivity) || apply subtype_trans with a0; assumption. Qed.
+Global Instance Top_otype: Top1 otype := fun _ top => Ot true top.
+Global Instance Bottom_otype: Bottom1 otype := fun _ bottom => Ot false bottom.
+Global Instance IsValidType_otype: IsValidType1 otype := @OType_Forall.
+Global Instance SubtypeRefl_otype: SubtypeRefl1 otype.
+Proof. intros A S V C a; destruct a; constructor; [destruct optional; simpl; reflexivity | apply subtype_refl]; inv H; assumption. Qed.
+Global Instance SubtypeAntisym_otype: SubtypeAntisym1 otype.
+Proof. intros A S E C a b H H0; destruct a, b; inv H H0; destruct optional, optional0; try discriminate; constructor; apply subtype_antisym; assumption. Qed.
+Global Instance SubtypeTrans_otype: SubtypeTrans1 otype.
+Proof. intros A S C a b c H H0; destruct a, b, c; inv H H0; destruct optional, optional0, optional1; try discriminate; constructor; (simpl; reflexivity) || apply subtype_trans with a0; assumption. Qed.
 
-Global Instance IsValidType_vtype {A: Set} `{V: IsValidType A}: IsValidType (vtype A) := fun a => match a with | VVoid => True | Vt a => V a end.
-Global Instance SubtypeRefl_vtype {A: Set} `{_SubtypeRefl: SubtypeRefl A}: SubtypeRefl (vtype A).
-Proof. intros a; destruct a; constructor; apply subtype_refl; assumption. Qed.
-Global Instance SubtypeAntisym_vtype {A: Set} `{_SubtypeAntisym: SubtypeAntisym A}: SubtypeAntisym (vtype A).
-Proof. intros a b H H0; destruct a, b; inv H H0; constructor; apply subtype_antisym; assumption. Qed.
-Global Instance SubtypeTrans_vtype {A: Set} `{_SubtypeTrans: SubtypeTrans A}: SubtypeTrans (vtype A).
-Proof. intros a b c H H0; destruct a, b, c; inv H H0; constructor; apply subtype_trans with a0; assumption. Qed.
+Global Instance IsValidType_vtype: IsValidType1 vtype := @VType_Forall.
+Global Instance SubtypeRefl_vtype: SubtypeRefl1 vtype.
+Proof. intros A S V C a; destruct a; constructor; apply subtype_refl; inv H; assumption. Qed.
+Global Instance SubtypeAntisym_vtype: SubtypeAntisym1 vtype.
+Proof. intros A S E C a b H H0; destruct a, b; inv H H0; constructor; apply subtype_antisym; assumption. Qed.
+Global Instance SubtypeTrans_vtype: SubtypeTrans1 vtype.
+Proof. intros A S C a b c H H0; destruct a, b, c; inv H H0; constructor; apply subtype_trans with a0; assumption. Qed.
 
-Global Instance IsValidType_tparam {A: Set} `{V: IsValidType A}: IsValidType (tparam A) := fun '(TParam _ _ supers) => @IsValidType_list A V supers.
-Global Instance SubtypeRefl_tparam {A: Set} `{_SubtypeRefl: SubtypeRefl A}: SubtypeRefl (tparam A).
-Proof. intros a; destruct a; constructor; apply subtype_refl; [reflexivity | assumption]. Qed.
-Global Instance SubtypeAntisym_tparam {A: Set} `{_SubtypeAntisym: SubtypeAntisym A}: SubtypeAntisym (tparam A).
-Proof. intros a b H H0; destruct a, b; inv H H0; rewrite (SubtypeAntisym_variance H2 H3); constructor; apply SubtypeAntisym_Intersect; assumption. Qed.
-Global Instance SubtypeTrans_tparam {A: Set} `{_SubtypeTrans: SubtypeTrans A}: SubtypeTrans (tparam A).
-Proof. intros a b c H H0; destruct a, b, c; inv H H0; constructor; [apply subtype_trans with v0 | apply subtype_trans with supers0]; assumption. Qed.
+Global Instance IsValidType_tparam: IsValidType1 tparam := @TParam_Forall.
+Global Instance SubtypeRefl_tparam: SubtypeRefl1 tparam.
+Proof. intros A S V C a; destruct a; constructor; [apply subtype_refl | apply (SubtypeRefl_Intersect subtype_refl)]; [reflexivity | inv H; assumption]. Qed.
+Global Instance SubtypeAntisym_tparam: SubtypeAntisym1 tparam.
+Proof. intros A S E C a b H H0; destruct a, b; inv H H0; rewrite (SubtypeAntisym_variance H2 H3); constructor; apply (SubtypeAntisym_Intersect subtype_antisym); assumption. Qed.
+Global Instance SubtypeTrans_tparam: SubtypeTrans1 tparam.
+Proof. intros A S C a b c H H0; destruct a, b, c; inv H H0; constructor; [apply subtype_trans with v0 | apply (SubtypeTrans_Intersect subtype_trans) with supers0]; assumption. Qed.
 
-Global Instance IsValidType_itype {A: Set} `{V: IsValidType A}: IsValidType (itype A) := fun '(It _ targs) => @IsValidType_list A V targs.
-Global Instance SubtypeRefl_itype {A: Set} `{_SubtypeRefl: SubtypeRefl A}: SubtypeRefl (itype A).
-Proof. intros a; destruct a; constructor; apply subtype_refl; assumption. Qed.
-Global Instance SubtypeAntisym_itype {A: Set} `{_SubtypeAntisym: SubtypeAntisym A}: SubtypeAntisym (itype A).
-Proof. intros a b H H0; destruct a, b; inv H H0; constructor; apply SubtypeAntisym_Zip; assumption. Qed.
-Global Instance SubtypeTrans_itype {A: Set} `{_SubtypeTrans: SubtypeTrans A}: SubtypeTrans (itype A).
-Proof. intros a b c H H0; destruct a, b, c; inv H H0; constructor; apply subtype_trans with targs0; assumption. Qed.
+Global Instance IsValidType_itype: IsValidType1 itype := @IType_Forall.
+Global Instance SubtypeRefl_itype: SubtypeRefl1 itype.
+Proof. intros A S V C a; destruct a; constructor; apply (SubtypeRefl_Zip subtype_refl); inv H; assumption. Qed.
+Global Instance SubtypeAntisym_itype: SubtypeAntisym1 itype.
+Proof. intros A S E C a b H H0; destruct a, b; inv H H0; constructor; apply (SubtypeAntisym_Zip subtype_antisym); assumption. Qed.
+Global Instance SubtypeTrans_itype: SubtypeTrans1 itype.
+Proof. intros A S C a b c H H0; destruct a, b, c; inv H H0; constructor; apply (SubtypeTrans_Zip subtype_trans) with targs0; assumption. Qed.
 
-Global Instance IsValidType_stype {A: Set} `{V: IsValidType A}: IsValidType (stype A) := fun x => match x with
-| SFn tparams thisp params restp ret => is_valid_type tparams /\ is_valid_type thisp /\ is_valid_type params /\ is_valid_type restp /\ is_valid_type ret
-| SArray elem => is_valid_type elem
-| STuple elems => is_valid_type elems
-| SObject fields => is_valid_type fields
-end.
-Global Instance SubtypeRefl_stype {A: Set} `{_SubtypeRefl: SubtypeRefl A}: SubtypeRefl (stype A).
-Proof. intros a; destruct a; constructor; apply subtype_refl; unfold is_valid_type, IsValidType_stype in H; decompose [and] H; assumption. Qed.
-Global Instance SubtypeAntisym_stype {A: Set} `{_SubtypeAntisym: SubtypeAntisym A}: SubtypeAntisym (stype A).
-Proof. intros a b H H0; destruct a, b; inv H H0; constructor; apply subtype_antisym || apply SubtypeAntisym_Zip || apply SubtypeAntisym_JsrZip; assumption. Qed.
-Global Instance SubtypeTrans_stype {A: Set} `{_SubtypeTrans: SubtypeTrans A}: SubtypeTrans (stype A).
-Proof. intros a b c H H0; destruct a, b, c; inv H H0; constructor; eapply subtype_trans; eassumption. Qed.
+Global Instance IsValidType_stype: IsValidType1 stype := @SType_Forall'.
+Global Instance SubtypeRefl_stype: SubtypeRefl1 stype.
+Proof. intros A S V C a; destruct a; constructor; (apply subtype_refl || apply (SubtypeRefl_Zip (SubtypeRefl_tparam subtype_refl)) || apply (SubtypeRefl_Zip (SubtypeRefl_otype subtype_refl)) || apply (SubtypeRefl_JsrZip (SubtypeRefl_otype subtype_refl)) || apply (SubtypeRefl_vtype subtype_refl)); inv H; assumption || (eapply unIsValidType1'; eassumption). Qed.
+Global Instance SubtypeAntisym_stype: SubtypeAntisym1 stype.
+Proof. intros A S E C a b H H0; destruct a, b; inv H H0; constructor; (apply subtype_antisym || apply (SubtypeAntisym_Zip (SubtypeAntisym_tparam subtype_antisym)) || apply (SubtypeAntisym_Zip (SubtypeAntisym_otype subtype_antisym)) || apply (SubtypeAntisym_JsrZip (SubtypeAntisym_otype subtype_antisym)) || apply (SubtypeAntisym_vtype subtype_antisym)); assumption. Qed.
+Global Instance SubtypeTrans_stype: SubtypeTrans1 stype.
+Proof. intros A S C a b c H H0; destruct a, b, c; inv H H0; constructor; (eapply subtype_trans || eapply (SubtypeTrans_Zip (SubtypeTrans_tparam subtype_trans)) || eapply (SubtypeTrans_Zip (SubtypeTrans_otype subtype_trans)) || eapply (SubtypeTrans_JsrZip (SubtypeTrans_otype subtype_trans)) || eapply (SubtypeTrans_vtype subtype_trans)); eassumption.
+Unshelve. exact (SubtypeTrans_Zip (SubtypeTrans_tparam subtype_trans)). exact (SubtypeTrans_Zip (SubtypeTrans_otype subtype_trans)). exact (SubtypeTrans_vtype subtype_trans). exact (SubtypeTrans_Zip (SubtypeTrans_otype subtype_trans)). exact (SubtypeTrans_JsrZip (SubtypeTrans_otype subtype_trans)). Qed.
 
-Definition IsValidType_ftype (x: ftype): Prop.
-  induction x using ftype_ind'.
-  - exact True.
-  - exact True.
-  - apply (@IsValidType_stype ftype); assumption.
-  - apply and; [apply and |]; [apply (@IsValidType_itype ftype) | apply (@IsValidType_list iftype); [apply (@IsValidType_itype ftype) |] | apply (@IsValidType_option sftype); [apply (@IsValidType_stype ftype) |]]; assumption.
-Qed.
-
-From Equations Require Import Equations.
-Equations _IsValidType_ftype (x: ftype): Prop by wf (ftype_depth x) lt :=
-_IsValidType_ftype FAny := True;
-_IsValidType_ftype (FNever _) := True;
-_IsValidType_ftype (FStructural _ structure) := @IsValidType_stype ftype (fun a => _IsValidType_ftype a) structure;
-_IsValidType_ftype (FNominal _ id sids structure) := @IsValidType_itype ftype (fun a => _IsValidType_ftype a) id /\ @IsValidType_list iftype (@IsValidType_itype ftype (fun a => _IsValidType_ftype a)) sids /\ @IsValidType_option sftype (@IsValidType_stype ftype (fun a => _IsValidType_ftype a)) structure.
-Next Obligation. auto.
-Program Fixpoint _IsValidType_ftype (x: ftype) {measure (ftype_depth x)}: Prop := match x with
-| FAny => True
-| FNever _ => True
-| FStructural _ structure => @IsValidType_stype ftype (fun a => _IsValidType_ftype a) structure
-| FNominal _ id sids structure => @IsValidType_itype ftype (fun a => _IsValidType_ftype a) id /\ @IsValidType_list iftype (@IsValidType_itype ftype (fun a => _IsValidType_ftype a)) sids /\ @IsValidType_option sftype (@IsValidType_stype ftype (fun a => _IsValidType_ftype a))  structure
-end.
-Next Obligation. simpl.
-
+Inductive _IsValidType_ftype: ftype -> Prop :=
+| FAny: _IsValidType_ftype FAny
+| FNever: forall x, _IsValidType_ftype (FNever x)
+| FStructural: forall x structure, @IsValidType_stype ftype _IsValidType_ftype structure -> _IsValidType_ftype (FStructural x structure)
+| FNominal: forall x id sids structure, @IsValidType_itype ftype _IsValidType_ftype id -> @IsValidType_list iftype (@IsValidType_itype ftype _IsValidType_ftype) sids -> @IsValidType_option sftype (@IsValidType_stype ftype _IsValidType_ftype) structure -> _IsValidType_ftype (FNominal x id sids structure)
+.
 Global Instance IsValidType_ftype: IsValidType ftype := _IsValidType_ftype.
+Fixpoint SubtypeRefl_ftype (a: ftype) (V: is_valid_type a): a <: a.
+destruct a.
+- constructor.
+- destruct nullable; constructor; reflexivity.
+- constructor; inv V; [destruct nullable; reflexivity |]; apply subtype_refl1; assumption.
+- constructor; inv V; [destruct nullable; reflexivity | ..]; eapply subtype_refl1.
 Global Instance SubtypeRefl_ftype {A: Set}: SubtypeRefl ftype.
-Proof. intros a; destruct a; constructor; apply subtype_refl; unfold is_valid_type, IsValidType_ftype in H; decompose [and] H; assumption. Qed.
+Ltac inv_con :=
+  lazymatch goal with
+  | |- [S_variance] ?a <: ?b => destruct a; constructor
+  | H : ?P -> ?a, H0 : ?Q ?a |- [?R] ?a <: ?b => apply H; assumption
+  | H : ?P ?a, H0 : ?Q ?a |- [?R] ?a <: ?b => destruct a; inv H H0; constructor
+  end.
+Proof.
+  intros a; induction a using ftype_ind'; constructor || (destruct nullable; constructor); try (try destruct nullable; reflexivity).
+  - apply subtype_refl1.
+       constructor. apply subtype_refl. unfold is_valid_type, IsValidType_ftype in H; decompose [and] H; assumption. Qed.
 Global Instance SubtypeAntisym_ftype {A: Set}: SubtypeAntisym ftype.
 Proof. intros a b H H0; destruct a, b; inv H H0; constructor; apply subtype_antisym || apply SubtypeAntisym_Zip || apply SubtypeAntisym_JsrZip; assumption. Qed.
 Global Instance SubtypeTrans_ftype {A: Set}: SubtypeTrans ftype.
